Move to general state expansion to handle locals

Atomics.thy
@@ -10,36 +10,12 @@ Describe concepts the logic must know about atomic instructions.
 
 section \<open>Helper Definitions\<close>
 
-datatype 'c tree = Leaf 'c | Branch "'c tree" "'c tree"
-
-type_synonym ('b,'c) gpred = "('b \<times> 'c tree) set"
-type_synonym ('b,'c) pred = "('b \<times> 'c) set"
-type_synonym ('b,'c) rpred = "'b rel"
-
-definition leaf :: "('b \<times> 'c) set \<Rightarrow> ('b \<times> 'c tree) set"
-  where "leaf e \<equiv> {(g,Leaf l) | g l. (g,l) \<in> e}"
-
-definition left :: "('b \<times> 'c tree) set \<Rightarrow> ('b \<times> 'c tree) set"
-  where "left e \<equiv> {(g,Branch l r) | g l r. (g,l) \<in> e}"
-
-definition right :: "('b \<times> 'c tree) set \<Rightarrow> ('b \<times> 'c tree) set"
-  where "right e \<equiv> {(g,Branch l r) | g l r. (g,r) \<in> e}"
-
-definition leaf\<^sub>r :: "('b \<times> 'c) rel \<Rightarrow> ('b \<times> 'c tree) rel"
-  where "leaf\<^sub>r e \<equiv> {((g,Leaf l),(g', Leaf l')) | g g' l l'. ((g,l),(g',l')) \<in> e}"
-
-definition left\<^sub>r :: "('b \<times> 'c tree) rel \<Rightarrow> ('b \<times> 'c tree) rel"
-  where "left\<^sub>r e \<equiv> {((g,Branch l r),(g',Branch l' r)) | g g' l l' r. ((g,l),(g',l')) \<in> e}"
-
-definition right\<^sub>r :: "('b \<times> 'c tree) rel \<Rightarrow> ('b \<times> 'c tree) rel"
-  where "right\<^sub>r e \<equiv> {((g,Branch l r),(g', Branch l r')) | g g' l r r'. ((g,r),(g',r')) \<in> e}"
-
-definition any :: "('b) set \<Rightarrow> ('b \<times> 'c tree) set"
-  where "any e \<equiv> {(g,t) | t g. (g) \<in> e}"
+type_synonym ('b) pred = "('b) set"
+type_synonym ('b) rpred = "('b) rel"
 
 text \<open>Stability of a predicate across an environment step\<close>
-definition stable :: "('b,'c) rpred \<Rightarrow> ('b,'c) pred \<Rightarrow> bool"
-  where "stable R P \<equiv> \<forall>g l g'. (g,l) \<in> P \<longrightarrow> (g,g') \<in> R \<longrightarrow> (g',l) \<in> P"
+definition stable :: "('b) rpred \<Rightarrow> ('b) pred \<Rightarrow> bool"
+  where "stable R P \<equiv> \<forall>m m'. m \<in> P \<longrightarrow> (m,m') \<in> R \<longrightarrow> m' \<in> P"
 
 text \<open>Weakest precondition for a precondition and postrelation\<close>
 definition wp 
@@ -58,12 +34,12 @@ lemma stable_conjI [intro]:
   using assms by (auto simp: stable_def)
 
 lemma stable_transitive:
-  assumes "(g,g') \<in> R\<^sup>*" "(g,l) \<in> P" "stable R P"
-  shows "(g',l) \<in> P"
+  assumes "(m,m') \<in> R\<^sup>*" "m \<in> P" "stable R P"
+  shows "m' \<in> P"
   using assms by (induct rule: rtrancl.induct) (auto simp: stable_def)
 
 lemma stable_wp\<^sub>tI:
-  "stable R P \<Longrightarrow> P \<subseteq> wp UNIV (fullR (R\<^sup>*)) P"
+  "stable R P \<Longrightarrow> P \<subseteq> wp UNIV (R\<^sup>*) P"
   unfolding wp_def using stable_transitive by fast
 
 lemma [intro]:
@@ -72,21 +48,14 @@ lemma [intro]:
 
 section \<open>Atomic Properties\<close>
 
-locale atomic =
-  fixes vc :: "'a \<Rightarrow> ('b \<times> 'c) set"
-  and beh :: "'a \<Rightarrow> ('b \<times> 'c) rel"
-
-context atomic
-begin
-
 text \<open>Weakest precondition of a basic instruction, based on the locale's 
       verification conditions and behaviours.\<close>
-abbreviation wp\<^sub>\<alpha> :: "'a \<Rightarrow> ('b,'c) pred \<Rightarrow> ('b,'c) pred"
+abbreviation wp\<^sub>\<alpha> :: "('a,'b) basic \<Rightarrow> 'b pred \<Rightarrow> 'b pred"
   where "wp\<^sub>\<alpha> \<alpha> Q \<equiv> wp (vc \<alpha>) (beh \<alpha>) Q"
 
 text \<open>Weakest precondition of a program, only covering basic instructions, environment steps and 
       sequential composition as these are sufficient for the logic's checks.\<close>
-fun wp\<^sub>c :: "('a,'b,'c) com \<Rightarrow> ('b,'c) pred \<Rightarrow> ('b,'c) pred"
+fun wp\<^sub>c :: "('a,'b) com \<Rightarrow> 'b pred \<Rightarrow> 'b pred"
   where 
     "wp\<^sub>c (Basic \<alpha>) Q = wp\<^sub>\<alpha> \<alpha> Q" |
     "wp\<^sub>c (Rel r) Q = wp UNIV r Q" |
@@ -94,28 +63,21 @@ fun wp\<^sub>c :: "('a,'b,'c) com \<Rightarrow> ('b,'c) pred \<Rightarrow> ('b,'
     "wp\<^sub>c _ Q = undefined"
 
 text \<open>Refinement relation between two programs, in terms of their weakest precondition calculation.\<close>
-definition refine :: "('a,'b,'c) com \<Rightarrow> ('a,'b,'c) com \<Rightarrow> bool" (infix "\<sqsubseteq>" 60)
+definition refine :: "('a,'b) com \<Rightarrow> ('a,'b) com \<Rightarrow> bool" (infix "\<sqsubseteq>" 60)
   where "c \<sqsubseteq> c' \<equiv> \<forall>Q. wp\<^sub>c c Q \<subseteq> wp\<^sub>c c' Q"
 
 text \<open>Merge the verification condition and behaviour to define evaluation\<close>
-definition eval :: "'a \<Rightarrow> ('b \<times> 'c) rel"
+definition eval :: "('a,'b) basic \<Rightarrow> 'b rel"
   where "eval \<alpha> \<equiv> {(m,m'). m \<in> vc \<alpha> \<longrightarrow> (m,m') \<in> beh \<alpha>}"
 
 text \<open>Specification check, ensuring an instruction conforms to a relation\<close>
-abbreviation guar :: "'a \<Rightarrow> ('b,'c) rpred \<Rightarrow> bool"
-  where "guar \<alpha> G \<equiv> {(g,g'). \<exists>l l'. (g,l) \<in> vc \<alpha> \<and> ((g,l),(g',l')) \<in> beh \<alpha>} \<subseteq> G\<^sup>="
-
-end
+abbreviation guar :: "('a,'b) basic \<Rightarrow> 'b rpred \<Rightarrow> bool"
+  where "guar \<alpha> G \<equiv> {(m,m'). m \<in> vc \<alpha> \<and> (m,m') \<in> beh \<alpha>} \<subseteq> G\<^sup>="
 
 section \<open>Atomic Rule\<close>
 
-locale atomic_rule = atomic
-
-context atomic_rule
-begin
-
 text \<open>Rule for an atomic operation\<close>
-definition atomic_rule :: "('b,'c) rpred \<Rightarrow> ('b,'c) rpred \<Rightarrow> ('b,'c) pred \<Rightarrow> 'a \<Rightarrow> ('b,'c) pred \<Rightarrow> bool" 
+definition atomic_rule :: "'b rpred \<Rightarrow> 'b rpred \<Rightarrow> 'b pred \<Rightarrow> ('a,'b) basic \<Rightarrow> 'b pred \<Rightarrow> bool" 
   ("_,_ \<turnstile>\<^sub>A _ {_} _" [40,0,0,0,40] 40)
   where "R,G \<turnstile>\<^sub>A P {\<alpha>} Q \<equiv> P \<subseteq> wp\<^sub>\<alpha> \<alpha> Q \<and> guar \<alpha> G \<and> stable R P \<and> stable R Q"
 
@@ -139,23 +101,84 @@ lemma actomic_conjI [intro]:
   shows "R,G \<turnstile>\<^sub>A P\<^sub>1 \<inter> P\<^sub>2 {\<alpha>} Q\<^sub>1 \<inter> Q\<^sub>2"
   using assms unfolding atomic_rule_def wp_def stable_def by fast
 
-(*
 text \<open>Add an invariant across an atomic judgement\<close>
-lemma atomic_frameI [intro]:
+lemma atomic_invI [intro]:
   assumes "R,G \<turnstile>\<^sub>A P {\<alpha>} Q"
-  assumes "stable R\<^sub>2 M" "G \<subseteq> R\<^sub>2"
-  shows "R \<inter> R\<^sub>2,G \<turnstile>\<^sub>A P \<inter> M {\<alpha>} Q \<inter> M"
+  assumes "stable R\<^sub>2 I" "G \<subseteq> R\<^sub>2"
+  shows "R \<inter> R\<^sub>2,G \<turnstile>\<^sub>A P \<inter> I {\<alpha>} Q \<inter> I"
   unfolding atomic_rule_def
 proof (safe, goal_cases)
-  case (1 g l)
-  hence "{(g,g'). \<exists>l l'. (g,l) \<in> P \<inter> vc \<alpha> \<and> ((g,l),(g',l')) \<in> beh \<alpha>} \<subseteq> R\<^sub>2\<^sup>=" "(g,l) \<in> vc \<alpha>"
+  case (1 m)
+  hence "{(m,m'). m \<in> P \<inter> vc \<alpha> \<and> (m,m') \<in> beh \<alpha>} \<subseteq> R\<^sub>2\<^sup>=" "m \<in> vc \<alpha>"
     using assms(1,3) by (auto simp: wp_def atomic_rule_def)
-  hence "(g,l) \<in> wp\<^sub>\<alpha> \<alpha> M" using assms(2) 1 by (auto simp: wp_def stable_def)
-  moreover have "(g,l) \<in> wp\<^sub>\<alpha> \<alpha> Q" using 1 assms(1) by (auto simp: atomic_rule_def wp_def)
+  hence "m \<in> wp\<^sub>\<alpha> \<alpha> I" using assms(2) 1 by (auto simp: wp_def stable_def)
+  moreover have "m \<in> wp\<^sub>\<alpha> \<alpha> Q" using 1 assms(1) by (auto simp: atomic_rule_def wp_def)
   ultimately show ?case by (auto simp: wp_def)
 qed (insert assms, auto simp: atomic_rule_def wp_def)
-*)
 
-end
+lemma atomic_falseI [intro]:
+  assumes "guar \<beta> G"
+  shows "R,G \<turnstile>\<^sub>A {} {\<beta>} {}"
+  using assms unfolding atomic_rule_def by auto
+
+section \<open>State Expansion\<close>
+
+definition expand\<^sub>P
+  where "expand\<^sub>P m P \<equiv> \<Union> (m ` P)"
+
+definition expand\<^sub>G
+  where "expand\<^sub>G m r G \<equiv> {(c,c'). \<exists>(b,b')\<in> G. c \<in> m b \<and> c' \<in> m b' \<and> r c c'}"
+
+definition expand\<^sub>R
+  where "expand\<^sub>R m R \<equiv> {(c,c'). \<exists>(b,b')\<in> R. c \<in> m b \<and> c' \<in> m b'}"
+
+definition valid_expand
+  where "valid_expand m r \<equiv> 
+          (\<forall>b b' c. c \<in> m b' \<longrightarrow> c \<in> m b \<longrightarrow> b = b') \<and> 
+          (\<forall>a b c. r a b \<longrightarrow> a \<in> m c \<longrightarrow> b \<in> m c \<longrightarrow> a = b)"
+
+lemma expand_stable:
+  assumes "stable R P" "valid_expand m r"
+  shows "stable (expand\<^sub>R m R) (expand\<^sub>P m P)"
+  using assms unfolding stable_def valid_expand_def expand\<^sub>P_def expand\<^sub>R_def
+  by fastforce
+
+lemma expand_wp\<^sub>\<alpha>:
+  assumes "P \<subseteq> wp\<^sub>\<alpha> \<alpha> Q" "valid_expand m r"
+  assumes \<alpha>: "vc \<alpha>' = expand\<^sub>P m (vc \<alpha>)" "beh \<alpha>' = expand\<^sub>G m r (beh \<alpha>)"
+  shows "expand\<^sub>P m P \<subseteq> wp\<^sub>\<alpha> \<alpha>' (expand\<^sub>P m Q)"
+  using assms(1,2) unfolding wp_def valid_expand_def expand\<^sub>P_def expand\<^sub>G_def \<alpha>
+  by fastforce
+
+lemma expand_guar:
+  assumes "guar \<alpha> G" "valid_expand m r"
+  assumes \<alpha>: "vc \<alpha>' = expand\<^sub>P m (vc \<alpha>)" "beh \<alpha>' = expand\<^sub>G m r (beh \<alpha>)"
+  shows "guar \<alpha>' (expand\<^sub>G m r G)"
+  using assms(1,2,3) unfolding valid_expand_def expand\<^sub>G_def \<alpha> expand\<^sub>P_def
+  by blast
+
+text \<open>Expand the state of an atomic judgement\<close>
+lemma atomic_expandI [intro]:
+  assumes "R,G \<turnstile>\<^sub>A P {\<alpha> :: ('b,'a) basic} Q"
+  assumes "valid_expand m r"
+  assumes \<alpha>: "vc \<alpha>' = expand\<^sub>P m (vc \<alpha>)" "beh \<alpha>' = expand\<^sub>G m r (beh \<alpha>)" 
+  shows "expand\<^sub>R m R,expand\<^sub>G m r G \<turnstile>\<^sub>A expand\<^sub>P m P {\<alpha>' :: ('b,'c) basic} expand\<^sub>P m Q"
+  unfolding atomic_rule_def
+proof (safe)
+  show "stable (expand\<^sub>R m R) (expand\<^sub>P m P)" 
+    using assms(1,2) expand_stable unfolding atomic_rule_def by blast
+next
+  show "stable (expand\<^sub>R m R) (expand\<^sub>P m Q)" 
+    using assms(1,2) expand_stable unfolding atomic_rule_def by blast
+next
+  fix x assume "x \<in> expand\<^sub>P m P"
+  thus "x \<in> wp\<^sub>\<alpha> \<alpha>' (expand\<^sub>P m Q)"
+    using assms(1,2) \<alpha> expand_wp\<^sub>\<alpha> unfolding atomic_rule_def by blast
+next
+  fix x x' assume b: "(x, x') \<notin> expand\<^sub>G m r G" "x \<in> vc \<alpha>'" "(x, x') \<in> beh \<alpha>'"
+  have "guar \<alpha>' (expand\<^sub>G m r G)"
+    using assms(1,2) \<alpha> expand_guar unfolding atomic_rule_def by blast
+  thus "x = x'" using b by auto
+qed
 
 end
