Interference.thy
@@ -21,17 +21,17 @@ text \<open>
 Independence of two instructions \<beta> and \<alpha> under environment R, 
 such that the early execution of \<alpha> is assumed to be possible and 
 cannot invalidate sequential reasoning.\<close>
-definition inter\<^sub>\<alpha> :: "('b,'c) rpred \<Rightarrow> ('b,'c) rpred \<Rightarrow> 'a \<Rightarrow> 'a \<Rightarrow> bool"
+definition inter\<^sub>\<alpha> :: "'b rpred \<Rightarrow> 'b rpred \<Rightarrow> ('a,'b) basic \<Rightarrow> ('a,'b) basic \<Rightarrow> bool"
   where "inter\<^sub>\<alpha> R G \<beta> \<alpha> \<equiv> 
-          Env R ; Basic \<beta> ; Env R ; Basic \<alpha> \<sqsubseteq> Env R ; Basic \<alpha>\<langle>\<beta>\<rangle> ; Env R ; Basic \<beta> \<and>
-          guar \<alpha>\<langle>\<beta>\<rangle> G"
+          Env R ; Basic \<beta> ; Env R ; Basic \<alpha> \<sqsubseteq> Env R ; Basic \<alpha>\<langle>tag \<beta>\<rangle> ; Env R ; Basic \<beta> \<and>
+          guar \<alpha>\<langle>tag \<beta>\<rangle> G"
 
 text \<open>
 Independence of program c and instruction \<alpha> under environment R,
 such that the early execution of \<alpha> is assumed to be possible and 
 cannot invalidate sequential reasoning.
 Define by recursively iterating over the program and capturing the forwarding throughout.\<close>
-fun inter\<^sub>c :: "('b,'c) rpred \<Rightarrow> ('b,'c) rpred \<Rightarrow> ('a,'b,'c) com \<Rightarrow> 'a \<Rightarrow> bool"
+fun inter\<^sub>c :: "'b rpred \<Rightarrow> 'b rpred \<Rightarrow> ('a,'b) com \<Rightarrow> ('a,'b) basic \<Rightarrow> bool"
   where
     "inter\<^sub>c R G (Basic \<beta>) \<alpha> = inter\<^sub>\<alpha> R G \<beta> \<alpha>" |
     "inter\<^sub>c R G (c\<^sub>1 ; c\<^sub>2) \<alpha> = (inter\<^sub>c R G c\<^sub>1 \<alpha>\<llangle>c\<^sub>2\<rrangle> \<and> inter\<^sub>c R G c\<^sub>2 \<alpha>)" |
